Most up-to-date to CN repo

CN_Lib/CN_Lib.lean
@@ -13,13 +13,13 @@ abbrev min_ULong : Int := 0
 abbrev max_ULong : Int := 2 ^ 64 - 1
 
 -- Bounds on the signed integer types.
-abbrev min_Char : Int := -(2 ^ 7 - 1)
+abbrev min_Char : Int := - (2 ^ 7)
 abbrev max_Char : Int := 2 ^ 7 - 1
-abbrev min_Short : Int := -(2 ^ 15 - 1)
+abbrev min_Short : Int := - (2 ^ 15)
 abbrev max_Short : Int := 2 ^ 15 - 1
-abbrev min_Int : Int := -(2 ^ 31 - 1)
+abbrev min_Int : Int := - (2 ^ 31)
 abbrev max_Int : Int := 2 ^ 31 - 1
-abbrev min_Long : Int := -(2 ^ 63 - 1)
+abbrev min_Long : Int := - (2 ^ 63)
 abbrev max_Long : Int := 2 ^ 63 - 1
 
 -- We roll our own pseudo-bitvectors below to match CN's representation of C
@@ -29,32 +29,32 @@ abbrev max_Long : Int := 2 ^ 63 - 1
 -- This function converts an integer to a vector of n bytes (represented as
 --    integers) in big-endian order.
 @[simp, reducible]
-def to_CN_BitVec (n : Nat) : Int → (Fin n → Int) :=
+def to_CN_Bytes (n : Nat) : Int → (Fin n → Int) :=
   fun v i => (v % 2 ^(8 * (n - i.toNat))) / (2 ^ (8 * (n - 1 - i.toNat)))
 @[simp, reducible]
-def from_CN_BitVec {n : Nat} (f : Fin n → Int) : Int :=
+def from_CN_Bytes {n : Nat} (f : Fin n → Int) : Int :=
   List.foldl
     (fun acc i => acc + f i * 2 ^ (8 * (n - 1 - i.toNat)))
     0
     (List.finRange n)
 
 @[simp, reducible]
-def UShort_bytes (v : Int) : Fin 2 → Int := to_CN_BitVec 2 v
+def UShort_bytes (v : Int) : Fin 2 → Int := to_CN_Bytes 2 v
 
 @[simp, reducible]
-def UInt_bytes (v : Int) : Fin 4 → Int := to_CN_BitVec 4 v
+def UInt_bytes (v : Int) : Fin 4 → Int := to_CN_Bytes 4 v
 
 @[simp, reducible]
-def ULong_bytes (v : Int) : Fin 8 → Int := to_CN_BitVec 8 v
+def ULong_bytes (v : Int) : Fin 8 → Int := to_CN_Bytes 8 v
 
 @[simp, reducible]
-def bytes_UShort (f : Fin 2 → Int) : Int := from_CN_BitVec f
+def bytes_UShort (f : Fin 2 → Int) : Int := from_CN_Bytes f
 
 @[simp, reducible]
-def bytes_UInt (f : Fin 4 → Int) : Int := from_CN_BitVec f
+def bytes_UInt (f : Fin 4 → Int) : Int := from_CN_Bytes f
 
 @[simp, reducible]
-def bytes_ULong (f : Fin 8 → Int) : Int := from_CN_BitVec f
+def bytes_ULong (f : Fin 8 → Int) : Int := from_CN_Bytes f
 
 theorem UShort_idem {v : Int} :
    min_UShort ≤ v ∧ v ≤ max_UShort
@@ -68,7 +68,7 @@ theorem UInt_idem {v : Int} :
   → v = bytes_UInt (UInt_bytes v) :=
 by
   intro ⟨Hv , Hv'⟩
-  unfold UInt_bytes  bytes_UInt from_CN_BitVec to_CN_BitVec List.finRange
+  unfold UInt_bytes  bytes_UInt from_CN_Bytes to_CN_Bytes List.finRange
   simp only [List.ofFn, Fin.foldr, Fin.foldr.loop, List.foldl]
   simp only [Fin.toNat]
   lia
@@ -78,7 +78,7 @@ theorem ULong_idem {v : Int} :
   → v = bytes_ULong (ULong_bytes v) :=
 by
   intro ⟨Hv , Hv'⟩
-  unfold ULong_bytes  bytes_ULong from_CN_BitVec to_CN_BitVec List.finRange
+  unfold ULong_bytes  bytes_ULong from_CN_Bytes to_CN_Bytes List.finRange
   simp only [List.ofFn, Fin.foldr, Fin.foldr.loop, List.foldl]
   simp only [Fin.toNat]
   lia
@@ -188,7 +188,7 @@ by
 
 theorem wrapI_pos_neg_neq :
   ∀ {max Umax v v' : Int} {_: Umax = 2 * max + 1},
-  0 ≤ v ∧ v ≤ max → -max ≤ v' ∧ v' < 0 →
+  0 ≤ v ∧ v ≤ max → -max - 1 ≤ v' ∧ v' < 0 →
   wrapI 0 Umax v ≠ wrapI 0 Umax v' :=
 by
   intros max Umax v v' inv Hv Hv'
@@ -204,7 +204,7 @@ by
   rw [hvrem, hvrem']; omega
 
 theorem wrapI_cong_pos :
-  ∀ {max Umax v v' : Int} {_ : 0 ≤ max}
+  ∀ {max Umax v v' : Int} {_ : 0 < max}
     {_ : Umax = (2 * max + 1)},
     0 ≤ v ∧ v ≤ max → 0 ≤ v' ∧ v' ≤ max
   → wrapI 0 Umax v = wrapI 0 Umax v'
@@ -218,9 +218,9 @@ by
   rw [HEq, HEq'] at Hwrap; assumption
 
 theorem wrapI_cong_neg :
-  ∀ {max Umax v v' : Int} {_ : 0 ≤ max}
+  ∀ {max Umax v v' : Int} {_ : 0 < max}
     {_ : Umax = (2 * max + 1)},
-    -max ≤ v ∧ v < 0 → -max ≤ v' ∧ v' < 0
+    -max - 1 ≤ v ∧ v < 0 → -max - 1 ≤ v' ∧ v' < 0
   → wrapI 0 Umax v = wrapI 0 Umax v'
   → v = v' :=
 by
@@ -242,8 +242,8 @@ by
   rw [hvrem, hvrem'] at hEq; omega
 
 theorem wrapI_cong :
-  ∀ {max v v' : Int}, 0 ≤ max
-  → -max ≤ v ∧ v ≤ max → -max ≤ v' ∧ v' ≤ max
+  ∀ {max v v' : Int}, 0 < max
+  → -max - 1 ≤ v ∧ v ≤ max → -max - 1 ≤ v' ∧ v' ≤ max
   → wrapI 0 (2 * max + 1) v = wrapI 0 (2 * max + 1) v'
   → v = v' :=
 by
@@ -255,14 +255,14 @@ by
       apply wrapI_cong_pos h h' Hwrap
       assumption; rfl
     · exfalso
-      have h' : -max ≤ v' ∧ v' < 0 := by omega
+      have h' : -max - 1 ≤ v' ∧ v' < 0 := by omega
       apply wrapI_pos_neg_neq h h' Hwrap; rfl
-  · have h : -max ≤ v ∧ v < 0 := by omega
+  · have h : -max - 1 ≤ v ∧ v < 0 := by omega
     by_cases h0' : 0 ≤ v'
     · exfalso
       have h' : 0 ≤ v' ∧ v' ≤ max := by omega
       apply wrapI_pos_neg_neq h' h Hwrap.symm; rfl
-    · have h' : -max ≤ v' ∧ v' < 0 := by omega
+    · have h' : -max - 1 ≤ v' ∧ v' < 0 := by omega
       apply wrapI_cong_neg h h' Hwrap
       assumption; rfl
 
@@ -273,7 +273,7 @@ theorem wrapI_Char_cong :
   → v = v' :=
 by
   intro Hv Hv' Hwrap
-  apply wrapI_cong _ Hv Hv' Hwrap; omega
+  apply wrapI_cong (max := max_Char) (by lia) Hv Hv' Hwrap
 
 theorem wrapI_Short_cong :
   min_Short ≤ v ∧ v ≤ max_Short
@@ -282,7 +282,7 @@ theorem wrapI_Short_cong :
   → v = v' :=
 by
   intro Hv Hv' Hwrap
-  apply wrapI_cong _ Hv Hv' Hwrap; omega
+  apply wrapI_cong (max := max_Short) (by lia) Hv Hv' Hwrap
 
 theorem wrapI_Int_cong :
   min_Int ≤ v ∧ v ≤ max_Int
@@ -291,7 +291,7 @@ theorem wrapI_Int_cong :
   → v = v' :=
 by
   intro Hv Hv' Hwrap
-  apply wrapI_cong _ Hv Hv' Hwrap; omega
+  apply wrapI_cong (max := max_Int) (by lia) Hv Hv' Hwrap
 
 theorem wrapI_Long_cong :
   min_Long ≤ v ∧ v ≤ max_Long
@@ -300,4 +300,4 @@ theorem wrapI_Long_cong :
   → v = v' :=
 by
   intro Hv Hv' Hwrap
-  apply wrapI_cong _ Hv Hv' Hwrap; omega
+  apply wrapI_cong (max := max_Long) (by lia) Hv Hv' Hwrap
